Switch to closed-world polymorphism encoding
Turns out true polymorphism was much worse, as was said by many people
online.

This also finishes the proof of Result 2, which is now much easier
without true polymorphism.

src/Language.v
@@ -96,6 +96,19 @@ Definition hat (aT : aliasedType) : ponyType :=
     | aType s b   => type s (base b)
   end.
 
+Lemma hat_preserves_type_id :
+  forall S S' : typeId,
+  forall b : baseCapability,
+  forall k : capability,
+  hat (aType S b) = type S' k
+    -> S = S'.
+Proof.
+  intros S S' b k.
+  (* Case analysis of b, compute the value of hat, introduce the hat equality,
+  * argue by constructors that the type IDs are equal *)
+  destruct b; compute; intro H; inversion H; reflexivity.
+  Qed.
+
 Inductive var : Type :=
   | variable : string -> var.
 
@@ -146,26 +159,15 @@ Inductive expressionSeq : Type :=
   | final : path -> expressionSeq
   | seq : expression -> expressionSeq -> expressionSeq.
 
-(* At several points, our proofs rely on the fact that the syntax types are distinct
- * (because I abuse polymorphism) - but in Coq, type inequalites are not provable
- * (in general) so we have to axiomatize the type inequalities we rely on *)
+(* Closed-world encoding used for polymorphic judgements *)
+Inductive cw_encoding : Type :=
+  | ePath : path -> cw_encoding
+  | eFieldOfPath : fieldOfPath -> cw_encoding
+  | eAlias : cw_encoding -> cw_encoding
+  | eExpr : expression -> cw_encoding
+  | eRhs : rhs -> cw_encoding.
 
-(* The antivalence axiom is not complete, but should eventually generate these *)
-Axiom fieldOfPath_ne_path : fieldOfPath <> path.
-Axiom aliased_ne_path : forall X : Type, @aliased X <> path.
-Axiom expr_ne_path : expression <> path. 
-Axiom rhs_ne_path : rhs <> path. 
-Axiom expr_ne_fieldOfPath : expression <> fieldOfPath.
-Axiom expr_ne_aliased : forall X : Type, @aliased X <> expression.
-Axiom expr_ne_rhs : expression <> rhs.
-
-Hint Resolve fieldOfPath_ne_path : core.
-Hint Resolve aliased_ne_path : core.
-Hint Resolve expr_ne_path : core.
-Hint Resolve rhs_ne_path : core.
-Hint Resolve expr_ne_fieldOfPath : core.
-Hint Resolve expr_ne_aliased : core.
-Hint Resolve expr_ne_rhs : core.
+Definition eAPaths (aPaths : list (@aliased path)) : list cw_encoding := map (fun ap => match ap with | aliasOf p =>  eAlias (ePath p) end) aPaths.
 
 End Syntax.
 
