src/Semantics.v
@@ -11,59 +11,58 @@ Module WFExpr := WFExpressions Map SetM.
 Module Heap := Heap Map.
 Include Heap.
 
-Inductive evaluatesTo { P : WFExpr.Program.program } : forall (X : Type), heap -> localVars -> X -> heap -> localVars -> value -> Prop :=
+Inductive evaluatesTo { P : WFExpr.Program.program } : heap -> localVars -> Syntax.cw_encoding -> heap -> localVars -> value -> Prop :=
   | eval_local (chi : heap) (L : localVars) (x : Syntax.var) (v : value)
   : LocalMap.VarMapsTo x v L
-    -> evaluatesTo Syntax.path chi L (Syntax.use x) chi L v
+    -> evaluatesTo chi L (Syntax.ePath (Syntax.use x)) chi L v
   | eval_temp (chi : heap) (L : localVars) (t : Syntax.temp) (v : value)
   : LocalMap.TempMapsTo t v L
-    -> evaluatesTo Syntax.path chi L (Syntax.useTemp t) chi (LocalMap.removeTemp t L) v
+    -> evaluatesTo chi L (Syntax.ePath (Syntax.useTemp t)) chi (LocalMap.removeTemp t L) v
   | eval_consume (chi : heap) (L : localVars) (x : Syntax.var) (v : value)
   : LocalMap.VarMapsTo x v L
-    -> evaluatesTo Syntax.path chi L (Syntax.consume x) chi (LocalMap.removeVar x L) v
+    -> evaluatesTo chi L (Syntax.ePath (Syntax.consume x)) chi (LocalMap.removeVar x L) v
   | eval_field (chi chi' : heap) (L L' : localVars) (p : Syntax.path) (f : Syntax.fieldId) (v v' : value)
-  : evaluatesTo Syntax.path chi L p chi' L' v
+  : evaluatesTo chi L (Syntax.ePath p) chi' L' v
     -> HeapFieldLookup v f v' chi'
-    -> evaluatesTo Syntax.fieldOfPath chi L (p, f) chi' L' v'
-  | eval_alias (chi chi' : heap) (L L' : localVars) (X : Type) (x : X) (v : value)
-  : evaluatesTo X chi L x chi' L' v
-    -> evaluatesTo (@Syntax.aliased X) chi L (Syntax.aliasOf x) chi' L' v
+    -> evaluatesTo chi L (Syntax.eFieldOfPath (p, f)) chi' L' v'
+  | eval_alias (chi chi' : heap) (L L' : localVars) (x : Syntax.cw_encoding) (v : value)
+  : evaluatesTo chi L x chi' L' v
+    -> evaluatesTo chi L (Syntax.eAlias x) chi' L' v
   | eval_vardecl (chi : heap) (L : localVars) (x : Syntax.var)
-  : evaluatesTo Syntax.expression chi L (Syntax.varDecl x) chi (LocalMap.addVar x None L) None
-  | eval_localassign (chi chi' : heap) (L L' : localVars) (x : Syntax.var) (arhs : @Syntax.aliased Syntax.rhs) (v v' : value)
-  : evaluatesTo Syntax.aliased chi L arhs chi' L' v
+  : evaluatesTo chi L (Syntax.eExpr (Syntax.varDecl x)) chi (LocalMap.addVar x None L) None
+  | eval_localassign (chi chi' : heap) (L L' : localVars) (x : Syntax.var) (rhs : Syntax.rhs) (v v' : value)
+  : evaluatesTo chi L (Syntax.eAlias (Syntax.eRhs rhs)) chi' L' v
     -> LocalMap.VarMapsTo x v' L'
-    -> evaluatesTo Syntax.expression chi L (Syntax.assign x arhs) chi' (LocalMap.addVar x v L') v'
-  | eval_fieldassign (chi chi' chi'' chi''' : heap) (L L' L'' : localVars) (p : Syntax.path) (f : Syntax.fieldId)
-    (ap : @Syntax.aliased Syntax.path) (u v v' : value)
-  : evaluatesTo Syntax.aliased chi L ap chi' L' v
-    -> evaluatesTo Syntax.path chi' L' p chi'' L'' u
+    -> evaluatesTo chi L (Syntax.eExpr (Syntax.assign x (Syntax.aliasOf rhs))) chi' (LocalMap.addVar x v L') v'
+  | eval_fieldassign (chi chi' chi'' chi''' : heap) (L L' L'' : localVars) (p p' : Syntax.path) (f : Syntax.fieldId)
+    (u v v' : value)
+  : evaluatesTo chi L (Syntax.eAlias (Syntax.ePath p')) chi' L' v
+    -> evaluatesTo chi' L' (Syntax.ePath p) chi'' L'' u
     -> HeapFieldLookup u f v' chi''
     -> HeapFieldAdd u f v chi'' chi'''
-    -> evaluatesTo Syntax.rhs chi L (Syntax.fieldAssign (p, f) ap) chi''' L'' v'
-  | eval_becall (chi chi' chi'' chi''' : heap) (L L' L'' : localVars) (rcvr : @Syntax.aliased Syntax.path) (args : list (@Syntax.aliased Syntax.path))
+    -> evaluatesTo chi L (Syntax.eRhs (Syntax.fieldAssign (p, f) (Syntax.aliasOf p'))) chi''' L'' v'
+  | eval_becall (chi chi' chi'' chi''' : heap) (L L' L'' : localVars) (rcvr : Syntax.path) (args : list (@Syntax.aliased Syntax.path))
     (b : Syntax.behaviourId) (rcvrVal : value) (argVals : list value)
-  : evaluatesTo_list Syntax.aliased chi L args chi' L' argVals
-    -> evaluatesTo Syntax.aliased chi' L' rcvr chi'' L'' rcvrVal
+  : evaluatesTo_list chi L (Syntax.eAPaths args) chi' L' argVals
+    -> evaluatesTo chi' L' (Syntax.eAlias (Syntax.ePath rcvr)) chi'' L'' rcvrVal
     -> False (*TODO: receiver is actor in the heap - is this necessary? *)
     -> HeapMessageAppend rcvrVal b argVals chi'' chi'''
-    -> evaluatesTo Syntax.rhs chi L (Syntax.behaviourCall rcvr b args) chi''' L'' rcvrVal
+    -> evaluatesTo chi L (Syntax.eRhs (Syntax.behaviourCall (Syntax.aliasOf rcvr) b args)) chi''' L'' rcvrVal
 with
-evaluatesTo_list { P : WFExpr.Program.program } : forall (X : Type), heap -> localVars -> list X -> heap -> localVars -> list value -> Prop :=
-  | evaluatesTo_list_nil (X : Type) (chi : heap) (L : localVars)
-  : evaluatesTo_list X chi L nil chi L nil
-  | evaluatesTo_list_cons (X: Type) (chi chi' chi'' : heap) (L L' L'' : localVars) (x : X) (lx : list X) (v : value) (lv : list value)
-  : evaluatesTo X chi L x chi' L' v
-    -> evaluatesTo_list X chi' L' lx chi'' L'' lv
-    -> evaluatesTo_list X chi L (x :: lx) chi'' L'' (v :: lv).
+evaluatesTo_list { P : WFExpr.Program.program } : heap -> localVars -> list Syntax.cw_encoding -> heap -> localVars -> list value -> Prop :=
+  | evaluatesTo_list_nil (chi : heap) (L : localVars)
+  : evaluatesTo_list chi L nil chi L nil
+  | evaluatesTo_list_cons (chi chi' chi'' : heap) (L L' L'' : localVars) (x : Syntax.cw_encoding)
+    (lx : list Syntax.cw_encoding) (v : value) (lv : list value)
+  : evaluatesTo chi L x chi' L' v
+    -> evaluatesTo_list chi' L' lx chi'' L'' lv
+    -> evaluatesTo_list chi L (x :: lx) chi'' L'' (v :: lv).
 
-Lemma paths_dont_change_heap { P : WFExpr.Program.program } : forall chi chi' L L' p v, @evaluatesTo P Syntax.path chi L p chi' L' v -> chi = chi'.
+Lemma paths_dont_change_heap { P : WFExpr.Program.program } : forall chi chi' L L' p v, @evaluatesTo P chi L (Syntax.ePath p) chi' L' v -> chi = chi'.
 Proof.
   intros.
-  (* Either the result is trivial *)
-  inversion H; try reflexivity.
-  (* Or there is a contradictory type equality in the hypotheses *)
-  all: try contradict H0; auto.
+  (* This is true by construction, so just invert and say so *)
+  inversion H; reflexivity.
   Qed.
 
 End Semantics.
